Silean2/Contracts.lean
@@ -1,4 +1,6 @@
 import Silean2.Contracts.NoResetFifo
+import Silean2.ModuleResetContract
+import Silean2.ModuleResetCertified
 import Silean2.Contracts.NoResetFifoExecution
 import Silean2.Contracts.NoResetFifoSerial
 import Silean2.Contracts.NoResetFifoView
