Silean2/Foundation.lean
@@ -1,6 +1,7 @@
 import Silean2.Foundation.SignalType
 import Silean2.Foundation.Enumeration
 import Silean2.Foundation.SignalMap
+import Silean2.Foundation.SignalExpectation
 import Silean2.Foundation.SignalSelection
 import Silean2.Foundation.ModulePorts
 import Silean2.Foundation.StructuralState
